code/experimental/rsapss/Hacl.Impl.Lib.fst
@@ -36,7 +36,7 @@ val le_u64: a:uint64 -> b:uint64 -> Tot bool
 let le_u64 a b = FStar.UInt64.(u64_to_UInt64 a <=^ u64_to_UInt64 b)
 
 inline_for_extraction noextract
-val eq_u8: a:uint8 -> b:uint8 -> Tot bool
+val eq_u8: a:uint8 -> b:uint8 -> Tot (r:bool{r == (uint_to_nat a = uint_to_nat b)})
 let eq_u8 a b = FStar.UInt8.(u8_to_UInt8 a =^ u8_to_UInt8 b)
 
 (* check if input[ind] is equal to 1 *)
